proof/garble/advGarble.ec
@@ -1,0 +1,267 @@
+require import Bitstring.
+require import Int.
+require import Bool.
+require import Pair.
+require import Map.
+require import Distr.
+require import List.
+require import Array.
+
+require import Dkc.
+require import Garble.
+require import GarbleTools.
+
+op eval(f:funct, i:input, k:int) = (evalComplete f i extract).[k].
+op void = (Bitstring.zeros 0).
+
+module Adv(A:Garble.Adv) : Dkc.Adv = {
+  var c : bool
+  var fc : Garble.funct
+  var xc : Garble.input
+  var good : bool
+  var tau : bool
+  var l : int
+  var queries : Dkc.query array
+  var ans : Dkc.answer array
+  var answer : Garble.functG*Garble.inputG*Garble.keyOutput
+  var query : Garble.query
+
+  var n : int
+  var m : int
+  var q : int
+  var aa : w2g
+  var bb : w2g
+  var gg : bool g2v
+  var pp : token g2v
+  var t : bool array
+  var v : bool array
+  var yy : token array
+  var xx : tokens
+  var a : int
+  var b : int
+  var i : int
+  var g : int
+
+  fun _query1(rand:bool, alpha:bool, bet:bool) : Dkc.query = {
+    var ttt : token;
+    var gamma : bool;
+    var pos : bool;
+    var input : int*bool;
+    var output : int*bool;
+    var ra : bool;
+    ttt = tweak g (t.[a]^^alpha) (t.[b]^^bet);
+    gamma = v.[g]^^(evalGate gg.[g] ((v.[a]^^alpha),(v.[b]^^alpha)));
+    if (a = l) {
+      pos = true;
+      input = (b, (t.[b]^^bet));
+    } else {
+      pos = false;
+      input = (a, (t.[a]^^alpha));
+    }
+    if (rand) {
+      ra = $Dbool.dbool;
+      output = (g + n + q, ra);
+    } else
+      output = (g, (t.[g]^^gamma));
+    return (input, output, pos, ttt);
+  }
+
+  fun _query2(rand:bool, alpha:bool, bet:bool, answer:Dkc.answer) : token = {
+    var gamma : bool;
+    var ki : token;
+    var ko : token;
+    var zz : token;
+    gamma = v.[g]^^(evalGate gg.[g] ((v.[a]^^alpha),(v.[b]^^alpha)));
+    (ki, ko, zz) = answer;
+    pp.[g] = setGateVal pp.[g] ((t.[a]^^alpha), (t.[b]^^bet)) zz;
+    if (a=l)
+      xx = setTok xx g (v.[b]^^bet) ki;
+    else
+      xx = setTok xx g (v.[a]^^alpha) ki;
+    if (! rand)
+      xx = setTok xx g (v.[g]^^gamma) ko;
+    return ko;
+  }
+
+  fun query1(rand:bool, alpha:bool, bet:bool) : unit = {
+    var query:Dkc.query;
+    query := _query1(rand, alpha, bet);
+    queries = query::queries;
+  }   
+
+  fun query2(rand:bool, alpha:bool, bet:bool) : token = {
+    var a:Dkc.answer;
+    var r:token;
+    a = ans.[(length ans) - 1];
+    ans = sub ans 0 ((length ans) - 1);
+    r := _query2(rand, alpha, bet, a);
+    return r;
+  }
+
+  fun query(rand:bool, alpha:bool, bet:bool) : token = {
+    var q:Dkc.query;
+    var a:Dkc.answer;
+    var r:token;
+    q := _query1(rand, alpha, bet);
+    (*a := DKC.encrypt(q);*)
+    r := _query2(rand, alpha, bet, a);
+    return r;
+  }
+
+  fun garb(yy:token, alpha:bool, bet:bool) : unit = {
+    pp.[g] = setGateVal pp.[g] ((t.[a]^^alpha), (t.[b]^^bet)) (Dkc.encode
+      (tweak g (t.[a]^^alpha) (t.[b]^^bet))
+      (getTok xx a (v.[a]^^alpha))
+      (getTok xx b (v.[b]^^alpha))
+      yy);
+  }
+
+  fun garbD(rand:bool, alpha:bool, bet:bool) : token = {
+    var yy : token;
+    if (rand)
+      yy = $Dkc.genRandKey;
+    else
+      yy = getTok xx g (evalGate gg.[g] ((v.[a]^^alpha),(v.[b]^^alpha)));
+    garb(yy, alpha, bet);
+    return yy;
+  }
+
+  fun garble_queries() : unit = {
+    i = 0;
+    while (i < n+q-1) {
+      t.[i] = eval fc xc i;
+      v.[i] = eval fc xc i;
+      i = i + 1;
+    }
+
+    i = 0;
+    while (i < n+q-m-1) {
+      t.[i] = $Dbool.dbool;
+      i = i + 1;
+    }
+
+    t.[l] = !tau;
+
+    g = n;
+    while (g < n+q-1) {
+      a = aa.[g];
+      b = bb.[g];
+      if (a = l) {
+        query1(false, true, false);
+        query1(false, true, true);
+      }
+      if (b = l) {
+        query1(false, false, true);
+        query1(true, true, true);
+      }
+      g = g + 1;
+    }
+  }
+
+  fun garble_answer() : unit = {
+    var tok : token;
+    var yyt : token;
+
+    g = n;
+    while (g < n+q-1) {
+      a = aa.[g];
+      b = bb.[g];
+      if (a = l) {
+        tok := query2(false, true, false);
+        tok := query2(false, true, true);
+      }
+      if (b = l) {
+        tok := query2(false, false, true);
+        yy.[g] := query2(true, true, true);
+      }
+      g = g + 1;
+    }
+
+    i = 0;
+    while (i < n+q-1) {
+      if (getTok xx i (!v.[i]) = void /\ i <> l) {
+        tok = $Dkc.genRandKeyLast (! t.[i]);
+        xx = setTok xx i (!v.[i]) tok;
+      }
+      if (getTok xx i (v.[i]) = void) {
+        tok = $Dkc.genRandKeyLast (t.[i]);
+        xx = setTok xx i (v.[i]) tok;
+      }
+      i = i + 1;
+    }
+
+    g = n;
+    while (g < n+q-1) {
+      a = aa.[g];
+      b = bb.[g];
+      garb(getTok xx g v.[g], false, false);
+      if (a <> l /\ b <> l) {
+        tok := garbD(a <= l, true, false);
+        tok := garbD(b <= l, false, true);
+        yyt := garbD(a <= l, true, true);
+        if (a <= l /\ l <= b /\ evalGate gg.[g] ((!v.[a]), false) = evalGate gg.[g] ((!v.[a]), true))
+          garb(yyt, true, false);
+      } else {
+        if (a = l) {
+          tok := garbD(false, false, true);
+        } else {
+          tok := garbD(true, true, false);
+          if (evalGate gg.[g] ((!v.[a]), false) = evalGate gg.[g] ((!v.[a]), true))
+            garb(yy.[g], true, false);
+        }
+      }
+      g = g + 1;
+    }
+    
+  }
+
+  
+  fun preInit() : unit = {
+    l = $Dinter.dinter 0 borne;
+  }
+
+  fun gen_queries(info:bool) : Dkc.query array = {
+    query := A.gen_query();
+    c = $Dbool.dbool;
+    if (c) {
+      fc = fst (fst query);
+      xc = snd (fst query);
+    } else {
+      fc = fst (snd query);
+      xc = snd (snd query);
+    }
+    (n, m, q, aa, bb, gg) = fc;
+    queries = Array.empty;
+    t = Array.init (n+q) false;
+    v = Array.init (n+q) false;
+    xx = Array.init (n+q) (void, void);
+    yy = Array.init (n+q) void;
+    gg = Array.init (n+q) (false, false, false, false);
+    pp = Array.init (n+q) (void, void, void, void);
+    tau = info;
+    if (Garble.queryValid query)
+    {
+      garble_queries();
+      good = true;
+    }
+    else
+      good = false;
+    return queries;
+  }
+  
+  fun get_challenge(answers:Dkc.answer array) : bool = {
+    var challenge : bool;
+    var ret : bool;
+    answers = answers;
+    if (good)
+    {
+      garble_answer();
+      challenge := A.get_challenge(answer);
+      ret = (c = challenge);
+    }
+    else
+      ret = $Dbool.dbool;
+    return ret;
+  }
+
+}.
