proof/garble/prFake.ec
@@ -1,0 +1,14 @@
+require import Bitstring.
+require import List.
+require import Map.
+require import Set.
+require import Pair.
+require import Real.
+require import Int.
+require import Bool.
+require import Array.
+
+require import Dkc.
+require import GarbleTools.
+require import Garble.
+require AdvGarble.
