proof/garble/prReal.ec
@@ -1,0 +1,70 @@
+require import Bitstring.
+require import List.
+require import Map.
+require import Set.
+require import Pair.
+require import Int.
+require import Bool.
+require import Array.
+require import Logic.
+
+require import Dkc.
+require import GarbleTools.
+require import Garble.
+require AdvGarble.
+
+
+
+lemma realEq :
+  forall (ADV <: Garble.Adv{AdvGarble.Adv}),
+    equiv [
+      Dkc.Game(Dkc.Dkc, AdvGarble.Adv(ADV)).work ~
+      Garble.Game(Garble.PrvInd(RandGarble), ADV).main
+      : (glob ADV){1} = (glob ADV){2} /\
+      (Dkc.Dkc.b{1}) /\ (AdvGarble.Adv.l{1}=0) ==> res{1} = res{2}
+    ]
+proof.
+
+  intros ADV.
+  fun.
+  inline {1} AdvGarble.Adv(ADV).gen_queries.
+  inline {1} AdvGarble.Adv(ADV).get_challenge.
+  inline {1} Dkc.Dkc.preInit.
+  inline {1} Dkc.Dkc.get_challenge.
+  inline {1} Dkc.Dkc.initialize.
+  inline {1} Dkc.Dkc.encrypt.
+  inline {1} AdvGarble.Adv(ADV).garble_queries.
+  inline {1} AdvGarble.Adv(ADV).garble_answer.
+  inline {1} AdvGarble.Adv(ADV).query1.
+  inline {1} AdvGarble.Adv(ADV).query2.
+  inline {1} AdvGarble.Adv(ADV)._query1.
+  inline {1} AdvGarble.Adv(ADV)._query2.
+  inline {1} AdvGarble.Adv(ADV).garb.
+  inline {1} AdvGarble.Adv(ADV).garbD.
+  inline {2} Garble.PrvInd(RandGarble).garb.
+  inline {2} Garble.PrvInd(RandGarble).get_challenge.
+  inline {2} RandGarble.gen.
+
+  swap{1} 7 -6.
+
+  app 1 1 : (AdvGarble.Adv.query{1} = query{2}).
+  call ((glob ADV){1} = (glob ADV){2}) (res{1}=res{2} /\ (glob ADV){1} = (glob ADV){2}).
+    fun true;trivial.
+  skip;trivial.
+  
+  case (Garble.queryValid query{2}).
+
+  rcondt {1} 18;[admit|].
+  rcondt {1} 33.
+  intros &m;kill 26!7. kill 1!24.
+wp;skip;trivial.
+wp.
+while true (AdvGarble.Adv.n + AdvGarble.Adv.q - 1 - AdvGarble.Adv.g). intros z.
+wp.
+kill 1!4.
+skip.
+trivial.
+if.
+  rcondt {2} 1;[intros &m;skip;trivial|].
+  
+save.
