proof/garble/proofGarble.ec
@@ -1,0 +1,227 @@
+require import Bitstring.
+require import List.
+require import Map.
+require import Set.
+require import Pair.
+require import Real.
+require import Int.
+require import Bool.
+require import Distr.
+require import Fun.
+require import Logic.
+
+require import Dkc.
+require import MyTools.
+require import Garble.
+require import GarbleTools.
+require AdvGarble.
+require import Mean.
+
+lemma prReal :
+  forall (ADV <: Garble.Adv{AdvGarble.Adv}),
+    forall &1 &2,
+      (glob ADV){1} = (glob ADV){2} /\
+      (Dkc.Dkc.b{1}) /\ (AdvGarble.Adv.l{1}=0) =>
+    Pr[Dkc.Game(Dkc.Dkc, AdvGarble.Adv(ADV)).work() @ &1 : res] =
+      Pr[Garble.Game(Garble.PrvInd(RandGarble), ADV).main() @ &2 : res]
+proof.
+  admit.
+save.
+
+lemma prHybrid :
+  forall (ADV <: Garble.Adv{AdvGarble.Adv}),
+    forall &1 &2,
+      (glob ADV){1} = (glob ADV){2} =>
+      (Dkc.Dkc.b{1}) /\ (!Dkc.Dkc.b{2}) =>
+      (AdvGarble.Adv.l{2}=AdvGarble.Adv.l{1}+1) =>
+    Pr[Dkc.Game(Dkc.Dkc, AdvGarble.Adv(ADV)).work() @ &1 : res] =
+      Pr[Dkc.Game(Dkc.Dkc, AdvGarble.Adv(ADV)).work() @ &2 : res]
+proof.
+  admit.
+save.
+
+lemma fakePr :
+  forall (ADV <: Garble.Adv{AdvGarble.Adv}),
+    forall &1,
+      (Dkc.Dkc.b{1}) /\ (AdvGarble.Adv.l{1}=borne) =>
+        Pr[Dkc.Game(Dkc.Dkc, AdvGarble.Adv(ADV)).work()@ &1 : res] = 1%r / 2%r
+proof.
+  admit.
+save.
+
+clone Mean as MeanBool with
+  type base = bool,
+  op d = Dbool.dbool,
+  op support = Set.add false (Set.add true Set.empty).
+clone Mean as MeanInt with
+  type base = int,
+  op d = Dinter.dinter 0 (borne-1).
+
+module AdvWork(Adv:Garble.Adv) : MeanInt.Worker = {
+  module Game = Dkc.Game(Dkc.Dkc, AdvGarble.Adv(Adv))
+  fun work(x:int) : bool = {
+    var r : bool;
+    AdvGarble.Adv.l = x;
+    r := Game.work();
+    return r;
+  }
+}.
+
+module DkcWork(Adv:Dkc.Adv) : MeanBool.Worker = {
+  module Game = Dkc.Game(Dkc.Dkc, Adv)
+  fun work(x:bool) : bool = {
+    var r : bool;
+    Dkc.Dkc.b = x;
+    Adv.preInit();
+    r := Game.work();
+    return r;
+  }
+}.
+
+module DkcWorkAdv(Adv:Dkc.Adv) = {
+  module Game = Dkc.Game(Dkc.Dkc, Adv)
+  fun work() : bool = {
+    var r : bool;
+    Adv.preInit();
+    r := Game.work();
+    return r;
+  }
+}.
+(*
+  axiom Rand :
+    forall &m,
+      forall (W<:Worker),
+        Pr[RandBit(W).randAndWork()@ &m:res] = fold_right
+          (lambda (x:base, sum:real), sum + (mu_x d x)*Pr[W.work(x)@ &m:res])
+          (0%r)
+          (support d).
+*)
+
+lemma AdvEsp :
+  forall &m,
+    forall (Adv<:Garble.Adv),
+      Pr[DkcWorkAdv(AdvGarble.Adv(Adv)).work()@ &m:res] =
+        (fold_right (lambda l x, x + (1%r / (borne-1)%r) * Pr[AdvWork(Adv).work(l)@ &m:res]) (0%r) MeanInt.support)
+proof.
+  intros &m Adv.
+  cut prelem : (forall (M<:Dkc.Exp), equiv[M.work~M.work:(glob M){1}=(glob M){2}==>res{1}=res{2}]);[intros M;fun true;trivial|].
+  cut lem : equiv[
+      MeanInt.Rand(AdvWork(Adv)).randAndWork ~
+      DkcWorkAdv(AdvGarble.Adv(Adv)).work: ((glob Dkc.Game(Dkc.Dkc, AdvGarble.Adv(Adv))){1}=(glob Dkc.Game(Dkc.Dkc, AdvGarble.Adv(Adv))){2})
+      ==>res{1}=res{2}].
+    fun.
+    inline AdvGarble.Adv(Adv).preInit.
+    inline AdvWork(Adv).work.
+    wp.
+    call ((glob Dkc.Game(Dkc.Dkc, AdvGarble.Adv(Adv))){1}=(glob Dkc.Game(Dkc.Dkc, AdvGarble.Adv(Adv))){2}) (res{1}=res{2}).
+      apply (prelem (<:Dkc.Game(Dkc.Dkc, AdvGarble.Adv(Adv)))).
+    wp.
+    rnd.
+    skip.
+    simplify.
+    intros &1 &2 h xL lR. split. clear h. trivial. intros heq hin.
+    (*elim h;clear h;intros h1 h2 h3.
+    split.
+    clear h3.
+    trivial.
+    clear h3.
+    apply h2.
+
+    elim h3;clear h3;intros h31 h32.
+    split.
+    split.
+    admit.
+    clear h31.
+    apply h32.
+    trivial.
+    apply h31.
+
+    apply h.*)
+
+    admit.
+
+  cut lem2 : (Pr[MeanInt.Rand(AdvWork(Adv)).randAndWork()@ &m:res] = Pr[DkcWorkAdv(AdvGarble.Adv(Adv)).work()@ &m:res]);[equiv_deno lem;trivial|].
+  rewrite <- lem2.
+  rewrite (_:
+(lambda (l : int) (x : real),
+     x +
+     (if in_supp l MeanInt.d then 1%r / (borne-1)%r else 0%r) *
+     Pr[AdvWork(Adv).work(l) @ &m : res])
+=
+(lambda (l : int) (x : real),
+     x +
+     (mu_x MeanInt.d l) *
+     Pr[AdvWork(Adv).work(l) @ &m : res])
+
+).
+
+  apply (Fun.extentionality<:real -> real, int>
+(lambda (l : int), lambda (x : real),
+     x +
+     (if in_supp l MeanInt.d then 1%r / (borne-1)%r else 0%r) *
+     Pr[AdvWork(Adv).work(l) @ &m : res])
+
+(lambda (l : int) (x : real),
+     x +
+     (mu_x MeanInt.d l) *
+     Pr[AdvWork(Adv).work(l) @ &m : res])
+_
+).
+intros l.
+
+  apply (Fun.extentionality<:real, real>
+(lambda (x : real),
+     x +
+     (if in_supp l MeanInt.d then 1%r / (borne-1)%r else 0%r) *
+     Pr[AdvWork(Adv).work(l) @ &m : res])
+
+(lambda (x : real),
+     x +
+     (mu_x MeanInt.d l) *
+     Pr[AdvWork(Adv).work(l) @ &m : res])
+_
+).
+intros x.
+rewrite (_:(mu_x MeanInt.d l=if in_supp l MeanInt.d then 1%r / (borne - 0 + 1)%r else 0%r)).
+case (in_supp l MeanInt.d).
+delta MeanInt.d.
+apply (Dinter.mu_x_def_in 0 borne l).
+trivial.
+delta MeanInt.d. delta mu_x.
+delta cPeq.
+simplify.
+trivial.
+apply (MeanInt.Mean &m (<:AdvWork(Adv))).
+save.
+
+lemma DkcEsp :
+  forall &m,
+    forall (Adv<:Dkc.Adv),
+      Pr[Dkc.Game(Dkc.Dkc, Adv).main()@ &m:res] = 
+        (Pr[DkcWork(Adv).work(true)@ &m:res] +
+           Pr[DkcWork(Adv).work(false)@ &m:res]) / 2%r
+proof.
+  admit.
+save.
+
+lemma RelDkcGarble :
+  forall &mDKC,
+    forall (Adv<:Garble.Adv),
+      forall &mGAR,
+      Pr[Garble.Game(Garble.PrvInd(RandGarble), Adv).main()@ &mGAR:res] =
+        2%r * borne%r * Pr[Dkc.Game(Dkc.Dkc, AdvGarble.Adv(Adv)).main()@ &mDKC:res]
+          + 1%r / 2%r - borne%r
+proof.
+  admit.
+save.
+
+lemma PrvIndGarble :
+  forall (epsilon:real),
+    forall (Adv<:Garble.Adv), forall &m,
+      epsilon > 0%r =>
+        Real.abs (Pr[Garble.Game(Garble.PrvInd(RandGarble), Adv).main()@ &m:res] - 1&r / 2%r) < epsilon
+proof.
+  admit.
+save.
+
+
