proof/gate/equivHybrid.ec
@@ -1,0 +1,205 @@
+require import Bitstring.
+require import List.
+require import Map.
+require import Set.
+require import Pair.
+require import Int.
+require import Real.
+require import Bool.
+
+require import Dkc.
+require import Gate.
+require import GarbleTools.
+require AdvGate.
+
+lemma hybridEq :
+      forall (Adv <: Gate.Adv{Dkc.Dkc, AdvGate.Adv}),
+        equiv [
+          Dkc.Game(Dkc.Dkc, AdvGate.Adv(Adv)).work ~
+            Dkc.Game(Dkc.Dkc, AdvGate.Adv(Adv)).work :
+          (glob Adv){1} = (glob Adv){2} /\
+          (!Dkc.Dkc.b{1}) /\ (AdvGate.Adv.l{1}=0) /\
+          (Dkc.Dkc.b{2}) /\ (AdvGate.Adv.l{2}=1)
+          ==> !res{1} = res{2}
+        ]
+proof.
+  intros Adv.
+  fun.
+  inline {1} Dkc.Dkc.preInit.
+  inline {1} Dkc.Dkc.get_challenge.
+  inline {1} Dkc.Dkc.initialize.
+  inline {1} AdvGate.Adv(Adv).gen_queries.
+  inline {1} AdvGate.Adv(Adv).get_challenge.
+  inline {1} AdvGate.Adv(Adv).compute0.
+  inline {1} AdvGate.Adv(Adv).gen_queries0.
+  inline {2} Dkc.Dkc.preInit.
+  inline {2} Dkc.Dkc.get_challenge.
+  inline {2} Dkc.Dkc.initialize.
+  inline {2} AdvGate.Adv(Adv).gen_queries.
+  inline {2} AdvGate.Adv(Adv).get_challenge.
+  inline {2} AdvGate.Adv(Adv).compute1.
+  inline {2} AdvGate.Adv(Adv).gen_queries1.
+ 
+  swap [7..9] -6.
+
+  app 3 3 : (
+    (glob Adv){1} = (glob Adv){2} /\
+    AdvGate.Adv.c{1} = AdvGate.Adv.c{2} /\
+    AdvGate.Adv.fc{1} = AdvGate.Adv.fc{2} /\
+    AdvGate.Adv.xc{1} = AdvGate.Adv.xc{2} /\
+    query{1} = query{2} /\
+    AdvGate.Adv.l{1}=0 /\
+    Dkc.Dkc.b{1} = false /\
+    AdvGate.Adv.l{2}=1 /\
+    Dkc.Dkc.b{2} = true
+  );
+[wp;call ((glob Adv){1} = (glob Adv){2}) ((glob Adv){1} = (glob Adv){2}/\res{1}=res{2});
+[fun true|rnd;skip];trivial|]. (* Call adv gen_queries *)
+
+  case (Gate.queryValid query{1}). (*good*)
+
+  rcondt {1} 9;[intros &m;wp;rnd;wp;rnd;skip;trivial|]. (*good*)
+  rcondf {1} 11;[admit|]. (* l condition *)
+  rcondt {1} 10;[admit|]. (* l condition *)
+  rcondt {1} 17;[intros &m;wp;rnd;wp;rnd;rnd;skip;admit|]. (* While *)
+  rcondt {1} 20;[admit|]. (* While *)
+  rcondf {1} 23;[admit|]. (* While *)
+  rcondt {1} 25;[admit|]. (* good *)
+  rcondf {1} 26;[admit|]. (* l *)
+  rcondt {1} 25;[admit|]. (* l *)
+
+  rcondt {2} 9;[intros &m;wp;rnd;wp;rnd;skip;trivial|]. (*good*)
+  rcondf {2} 10;[admit|]. (* l condition *)
+  rcondt {2} 10;[admit|]. (* l condition *)
+  rcondt {2} 18;[admit|]. (* While *)
+  rcondt {2} 21;[admit|]. (* While *)
+  rcondf {2} 24;[admit|]. (* While *)
+  rcondt {2} 26;[admit|]. (* good *)
+  rcondf {2} 26;[admit|]. (* l *)
+  rcondt {2} 26;[admit|]. (* l *)
+
+  inline {1} Dkc.Dkc.encrypt.
+  inline {2} Dkc.Dkc.encrypt.
+
+  (*BEGIN CLEAN DKC*)
+  (*LOOP 1*)
+  (rcondt {1} 20;[admit|]). (* Dkc used *)
+  (rcondt {1} 21;[admit|]). (* Dkc not reusing *)
+  (rcondt {1} 22;[admit|]). (* Dkc not reusing *)
+  (rcondt {1} 23;[admit|]). (* Dkc not reusing *)
+  (rcondt {2} 21;[admit|]). (* Dkc used *)
+  (rcondt {2} 22;[admit|]). (* Dkc not reusing *)
+  (rcondt {2} 23;[admit|]). (* Dkc not reusing *)
+  (rcondt {2} 24;[admit|]). (* Dkc not reusing *)
+  (*LOOP 2*)
+  (rcondt {1} 33;[admit|]). (* Dkc used *)
+  (rcondt {1} 34;[admit|]). (* Dkc not reusing *)
+  (rcondt {1} 35;[admit|]). (* Dkc not reusing *) (*TODO: FALSE*)
+  (rcondt {1} 36;[admit|]). (* Dkc not reusing *)
+  (rcondt {2} 34;[admit|]). (* Dkc used *)
+  (rcondt {2} 35;[admit|]). (* Dkc not reusing *)
+  (rcondt {2} 36;[admit|]). (* Dkc not reusing *)
+  (rcondt {2} 37;[admit|]). (* Dkc not reusing *)
+  (*END CLEAN DKC*)
+
+  wp.
+  call ((glob Adv){1} = (glob Adv){2}/\answer{1}=answer{2}) (res{1}=res{2}).
+    fun true;trivial.
+  wp.
+  (*
+  alias {1} 1 with _tau.
+  alias {1} 3 with _keytau.
+  alias {1} 12 with _t;swap {1} 12 -10.
+  alias {1} 24 with _keyt;swap {1} 24 -15.
+  alias {1} 25 with _key_tau_t;swap {1} 25 -25.
+
+  alias {2} 1 with nt.*)
+
+  (*init vals*)
+  swap [3..4] -2. (*maps*)
+  swap{1} [15..16] -12. (*i answers*)
+  swap{2} [16..17] -13. (*i answers*)
+  swap [9..10] -4. (*query*)
+  swap{1} 14 -13. (*good*)
+  swap{2} 15 -14. (*good*)
+  
+  (*tau{1}*)
+  swap{1} [10..12] -1. (*rewrite tau*)
+  swap{2} 13 -5. (*t*)
+
+  (*t{1}*)
+  swap{1} 13 -1. (*t*)
+  swap{2} [11..13] -1. (*rewrite tau*)
+
+
+  swap{1} [29..33] -8. (*init loop*)
+  swap{2} [30..34] -8. (*init loop*)
+
+  (*keytau{1}*)
+  swap{1} 13 12. (*keytau*)
+  alias{2} 35 with _keytau.
+  swap{2} 35 -8. (*keynt*)
+
+  (*keyt{1}*)
+  swap{2} 51 -23. (*keyntau*)
+
+  (*keyt{1}*)
+  swap{2} 51 -23. (*keyntau*)
+  
+
+  (*t{1}*)
+
+
+  swap{2} 10 -9. (*t*)
+  swap{2} [6..7] -3. (*rewrite tau*)
+  swap{2} 10 -5. (*rewrite tau*)
+
+
+
+
+
+  swap{2} 38 -31. (*keyntau*)
+
+  swap{2} 39 -30. (*key_nt_ntau*)
+  swap{2} 39 -25. (*keyntau*)
+  swap{1} 38 -25. (*keyntau*)
+  swap{1} 10 -8. (*t*)
+  swap{2} 11 -10. (*t*)
+
+
+  case (
+(Gate.eval AdvGate.Adv.fc{1} AdvGate.Adv.xc{1}=Gate.eval AdvGate.Adv.fc{1} (!(fst AdvGate.Adv.xc{1}), (snd AdvGate.Adv.xc{1}))) /\
+(Gate.eval AdvGate.Adv.fc{2} AdvGate.Adv.xc{2}=Gate.eval AdvGate.Adv.fc{2} (!(fst AdvGate.Adv.xc{2}), (snd AdvGate.Adv.xc{2})))
+).
+  rcondt{1} 37;[admit|].
+  rcondt{1} 38;[admit|].
+  rcondt{2} 39;[admit|].
+  wp.
+
+  (*BEGIN CLEAN DKC*)
+  (*LOOP 2*)
+  (rcondt {1} 28;[admit|]). (* Dkc used *)
+  (rcondt {1} 29;[admit|]). (* Dkc not reusing *)
+  (rcondt {1} 30;[admit|]). (* Dkc not reusing *) (*TODO: FALSE*)
+  (rcondt {1} 31;[admit|]). (* Dkc not reusing *)
+  (rcondt {2} 30;[admit|]). (* Dkc used *)
+  (rcondt {2} 31;[admit|]). (* Dkc not reusing *)
+  (rcondt {2} 32;[admit|]). (* Dkc not reusing *)
+  (rcondt {2} 33;[admit|]). (* Dkc not reusing *)
+  (*LOOP 1*)
+  (rcondt {1} 21;[admit|]). (* Dkc used *)
+  (rcondt {1} 22;[admit|]). (* Dkc not reusing *)
+  (rcondt {1} 23;[admit|]). (* Dkc not reusing *)
+  (rcondt {1} 24;[admit|]). (* Dkc not reusing *)
+  (rcondt {2} 23;[admit|]). (* Dkc used *)
+  (rcondt {2} 24;[admit|]). (* Dkc not reusing *)
+  (rcondt {2} 25;[admit|]). (* Dkc not reusing *)
+  (rcondt {2} 26;[admit|]). (* Dkc not reusing *)
+  (*END CLEAN DKC*)
+
+  wp.
+
+  rnd.
+  rnd.
+  swap{2} 37 -34.
+save.
