proof/mean.ec
@@ -1,0 +1,42 @@
+require import Set.
+require import Real.
+require import Distr.
+
+op fold_right : ('a -> 'b -> 'b) -> 'b -> 'a set -> 'b.
+axiom fold_nil: forall (e:'b) (f:'a -> 'b -> 'b),
+  fold_right f e Set.empty = e.
+axiom fold_cons: forall (e:'b) (f:'a -> 'b -> 'b) xs,
+  let x = Set.pick xs in
+  fold_right f e xs = f x (fold_right f e (Set.rm x xs)).
+
+theory Mean.
+  type base.
+
+  op d : base distr.
+  op support : base set.
+  axiom in_support :
+    forall (x:base, d:base distr),
+      in_supp x d <=> mem x support.
+  
+  module type Worker = {
+    fun work(x:base) : bool
+  }.
+
+  module Rand(W:Worker) = {
+    fun randAndWork() : bool = {
+      var r : bool;
+      var x : base;
+      x = $d;
+      r := W.work(x);
+      return r;
+    }
+  }.
+
+  axiom Mean :
+    forall &m,
+      forall (W<:Worker),
+        Pr[Rand(W).randAndWork()@ &m:res] = fold_right
+          (lambda (x:base, sum:real), sum + (mu_x d x)*Pr[W.work(x)@ &m:res])
+          (0%r)
+          support.
+end Mean.
